specs/Spec.SHA2.fst
@@ -32,54 +32,6 @@ inline_for_extraction
 let word_lognot: a:sha2_alg -> Tot ((word a) -> Tot (word a)) = function
   | SHA2_224 | SHA2_256 -> lognot #U32 #SEC
   | SHA2_384 | SHA2_512 -> lognot #U64 #SEC
-
-(*
-inline_for_extraction
-let word_add_mod: a:sha2_alg -> Tot ((word a) -> (word a) -> Tot (word a)) = function
-  | SHA2_224 | SHA2_256 -> add_mod #U32 #SEC
-  | SHA2_384 | SHA2_512 -> add_mod #U64 #SEC
-
-inline_for_extraction
-let word_logxor: a:sha2_alg -> Tot ((word a) -> (word a) -> Tot (word a)) = function
-  | SHA2_224 | SHA2_256 -> U32.logxor
-  | SHA2_384 | SHA2_512 -> U64.logxor
-
-inline_for_extraction
-let word_logand: a:sha2_alg -> Tot ((word a) -> (word a) -> Tot (word a)) = function
-  | SHA2_224 | SHA2_256 -> U32.logand
-  | SHA2_384 | SHA2_512 -> U64.logand
-
-inline_for_extraction
-let word_logor: a:sha2_alg -> Tot ((word a) -> (word a) -> Tot (word a)) = function
-  | SHA2_224 | SHA2_256 -> U32.logor
-  | SHA2_384 | SHA2_512 -> U64.logor
-
-inline_for_extraction
-let word_lognot: a:sha2_alg -> Tot ((word a) -> Tot (word a)) = function
-  | SHA2_224 | SHA2_256 -> U32.lognot
-  | SHA2_384 | SHA2_512 -> U64.lognot
-
-inline_for_extraction
-let word_shift_right: t:sha2_alg -> Tot (a:word t -> s:U32.t -> Pure (word t)
-  (requires (FStar.Mul.(U32.v s < 8 * word_length t)))
-  (ensures (fun c -> v' c = (v' a / (pow2 (U32.v s)))))) = function
-  | SHA2_224 | SHA2_256 -> U32.shift_right
-  | SHA2_384 | SHA2_512 -> U64.shift_right
-
-inline_for_extraction
-let rotate_right32 (x:U32.t) (s:U32.t{0 < U32.v s /\ U32.v s < 32}): Tot U32.t =
-  U32.((x >>^ s) |^ (x <<^ (32ul -^ s)))
-
-inline_for_extraction
-let rotate_right64 (a:U64.t) (s:U32.t{0 < U32.v s /\ U32.v s < 64}): Tot U64.t =
-  U64.((a >>^ s) |^ (a <<^ (U32.sub 64ul s)))
-
-inline_for_extraction
-let word_rotate_right: a:sha2_alg -> Tot (word a -> s:U32.t{0 < U32.v s /\ U32.v s < word_n a} -> Tot (word a)) = function
-  | SHA2_224 | SHA2_256 -> rotate_right32
-  | SHA2_384 | SHA2_512 -> rotate_right64
-
-*)
 inline_for_extraction noextract
 type ops = {
   c0: size_t; c1: size_t; c2: size_t;
